---
Related:
  - "[[Grenzwerte|Grenzwerte]]"
  - "[[Uneigentliche Grenzwerte]]"
---

> [!IMPORTANT] Satz: Rechenregeln für uneigentliche Grenzwerte
> 
> ||$\displaystyle \lim_{x\to c} f(x) = L \lt 0$|$\displaystyle \lim_{x\to c} f(x) = L \gt 0$|
> |:--:|:--:|:--:|
> |$\displaystyle \lim_{x\to c} g(x) = -\infty$|$\displaystyle \lim_{x\to c} (f(x) + g(x)) = -\infty$ </br> $\displaystyle\lim_{x\to c} (f(x)g(x)) = +\infty$|$\displaystyle \lim_{x\to c} (f(x) + g(x)) = -\infty$ </br> $\displaystyle\lim_{x\to c} (f(x)g(x)) = -\infty$|
> |$\displaystyle \lim_{x\to c} g(x) = + \infty$|$\displaystyle \lim_{x\to c} (f(x) + g(x)) = +\infty$ </br> $\displaystyle\lim_{x\to c} (f(x)g(x)) = -\infty$|$\displaystyle \lim_{x\to c} (f(x) + g(x)) = +\infty$ </br> $\displaystyle\lim_{x\to c} (f(x)g(x)) = +\infty$|
> 
> ||$\displaystyle \lim_{x\to c} f(x) = -\infty$|$\displaystyle \lim_{x\to c} f(x) = +\infty$|
> |:--:|:--:|:--:|
> |$\displaystyle \lim_{x\to c} g(x) = -\infty$|$\displaystyle \lim_{x\to c} (f(x) + g(x)) = -\infty$ </br> $\displaystyle\lim_{x\to c} (f(x)g(x)) = +\infty$|$\displaystyle \lim_{x\to c} (f(x) + g(x)) = \, ?$ </br> $\displaystyle\lim_{x\to c} (f(x)g(x)) = -\infty$|
> |$\displaystyle \lim_{x\to c} g(x) = + \infty$|$\displaystyle \lim_{x\to c} (f(x) + g(x)) = \, ?$ </br> $\displaystyle\lim_{x\to c} (f(x)g(x)) = -\infty$|$\displaystyle \lim_{x\to c} (f(x) + g(x)) = +\infty$ </br> $\displaystyle\lim_{x\to c} (f(x)g(x)) = +\infty$|
> 
> > [!NOTE]
> > Diese Regeln gelten auch für $x\to \pm \infty$.